src/TraverseOpImpl.v
@@ -16,29 +16,343 @@ Import ExpandMode.
 Import MatchMode.
 Import UpdateNotations.
 
+Require Import RAUtils.
+From RelationAlgebra Require Import syntax matrix bmx monoid sums boolean.
+Open Scope ra_terms.
+
+Section translate.
+  Variable G : PropertyGraph.t.
+  Notation V := (PropertyGraph.vertices G).
+  Notation E := (PropertyGraph.edges G).
+
+  Hypothesis Hwf_G : PropertyGraph.wf G.
+
+  Definition vertices_sup := S (\sup_(v \in V) v).
+
+  Definition edges_sup := S (\sup_(e \in E) e).
+
+  Definition adj_mat_ty := bmx vertices_sup vertices_sup.
+
+  Lemma vertex_ltb_vertices_sub v
+    (HIn : In v V) : v < vertices_sup.
+  Proof.
+    unfold vertices_sup.
+    apply ltb_succ.
+    change (v <= \sup_(v0 \in V) v0) with
+      (leq (id v) (sup id V)).
+    now apply leq_xsup.
+  Qed.
+
+  Lemma edge_ltb_edges_sub e
+    (HIn : In e E) : e < edges_sup.
+  Proof.
+    unfold edges_sup.
+    apply ltb_succ.
+    change (e <= \sup_(e0\in E) e0) with
+      (leq (id e) (sup id E)).
+    now apply leq_xsup.
+  Qed.
+
+  Definition ord_of_vertex (v : vertex)
+    (HIn : In v V) :
+      ord vertices_sup :=
+    Ord v (vertex_ltb_vertices_sub v HIn).
+
+  Definition ord_of_edge (e : edge)
+    (HIn : In e E) :
+      ord edges_sup :=
+    Ord e (edge_ltb_edges_sub e HIn).
+
+  Definition adj_matrix_of_edge (l : option label) (e : edge) : adj_mat_ty :=
+    fun i j => (e_from G e ==b i) &&
+               (e_to G e ==b j) &&
+               match l with
+               | Some l => (elabel G e ==b l)
+               | None => true
+               end.
+
+  Theorem adj_matrix_of_edge_spec e l i j :
+    adj_matrix_of_edge l e i j <->
+      Path.matches_direction G i j e Pattern.OUT /\
+      match l with
+      | Some l => elabel G e = l
+      | None => True
+      end.
+  Proof.
+    unfold adj_matrix_of_edge.
+    unfold is_true; desf.
+    all: repeat rewrite Bool.andb_true_iff.
+    all: repeat rewrite equiv_decb_true_iff.
+    all: simpl; unfold e_from, e_to; destruct (ends G e); simpl.
+    all: split; ins; desf.
+  Qed.
+
+  Definition adj_matrix (l : option label) : adj_mat_ty :=
+    (\sum_(e \in E) (adj_matrix_of_edge l e)).
+
+  Theorem adj_matrix_spec_OUT l i j :
+    adj_matrix l i j <-> exists e, In e E /\
+      Path.matches_direction G i j e Pattern.OUT /\
+      match l with
+      | Some l => elabel G e = l
+      | None => True
+      end.
+  Proof.
+    unfold adj_matrix.
+    setoid_rewrite <- adj_matrix_of_edge_spec.
+    rewrite <- is_true_sup.
+    now rewrite <- mx_sup.
+  Qed.
+
+  Theorem adj_matrix_spec_IN l i j :
+    adj_matrix l j i <-> exists e, In e E /\
+      Path.matches_direction G i j e Pattern.IN /\
+      match l with
+      | Some l => elabel G e = l
+      | None => True
+      end.
+  Proof.
+    simpl. apply adj_matrix_spec_OUT.
+  Qed.
+
+  Theorem adj_matrix_spec_BOTH l i j :
+    adj_matrix l i j || adj_matrix l j i <->
+      exists e, In e E /\
+        Path.matches_direction G i j e Pattern.BOTH /\
+        match l with
+        | Some l => elabel G e = l
+        | None => True
+        end.
+  Proof.
+    unfold is_true.
+    rewrite Bool.orb_true_iff.
+    change (?b = true) with (is_true b).
+    rewrite adj_matrix_spec_OUT.
+    rewrite adj_matrix_spec_IN.
+    split; ins; desf; eauto.
+  Qed.
+
+  Definition inc_mat_ty := bmx vertices_sup edges_sup.
+
+  Definition inc_matrix : inc_mat_ty :=
+    fun i j => (e_from G j ==b i).
+
+  Definition inc_matrix_inv : inc_mat_ty :=
+    fun i j => (e_to G j ==b i).
+
+  Theorem inc_matrix_spec i j :
+    inc_matrix i j <->
+      e_from G j = i.
+  Proof.
+    unfold inc_matrix.
+    unfold is_true.
+    now rewrite equiv_decb_true_iff.
+  Qed.
+
+  Theorem inc_matrix_inv_spec i j :
+    inc_matrix_inv i j <->
+      e_to G j = i.
+  Proof.
+    unfold inc_matrix_inv.
+    unfold is_true.
+    now rewrite equiv_decb_true_iff.
+  Qed.
+
+  Theorem inc_matrix_spec_OUT i j :
+    inc_matrix i j <->
+      Path.matches_direction G i (e_to G j) j Pattern.OUT.
+  Proof.
+    rewrite inc_matrix_spec.
+    simpl; unfold e_from, e_to; destruct (ends G j); simpl.
+    split; ins; desf.
+  Qed.
+
+  Theorem inc_matrix_inv_spec_IN i j :
+    inc_matrix_inv i j <->
+      Path.matches_direction G i (e_from G j) j Pattern.IN.
+  Proof.
+    rewrite inc_matrix_inv_spec.
+    simpl; unfold e_from, e_to; destruct (ends G j); simpl.
+    split; ins; desf.
+  Qed.
+
+  Definition label_matrix (l : label) : adj_mat_ty :=
+    fun i j => eqb i j && In_decb l (vlabels G i).
+
+  Theorem label_matrix_spec l i j :
+    label_matrix l i j <-> i = j /\ In l (vlabels G i).
+  Proof.
+    unfold label_matrix, is_true.
+    rewrite Bool.andb_true_iff, In_decb_true_iff.
+    case eqb_spec; split; ins; desf.
+  Qed.
+
+  Fixpoint translate_slice' (pi' : PatternSlice.t) : adj_mat_ty :=
+    match pi' with
+    | PatternSlice.empty => 1
+    | PatternSlice.hop pi' pe pv =>
+      let mpi' := translate_slice' pi' in
+      let mpe :=
+        let l := Pattern.elabel pe in
+          match Pattern.edir pe with
+          | Pattern.OUT => adj_matrix l
+          | Pattern.IN => (adj_matrix l)°
+          | Pattern.BOTH => (adj_matrix l) + (adj_matrix l)°
+          end
+      in
+      let mpv := 
+        let l := Pattern.vlabel pv in
+          match l with
+          | Some l => label_matrix l
+          | None => 1 (* identity matrix *)
+          end
+      in mpi' ⋅ mpe ⋅ mpv
+    end.
+
+  Lemma andb_is_true_iff a b :
+    a && b <-> a /\ b.
+  Proof.
+    unfold is_true.
+    now rewrite Bool.andb_true_iff.
+  Qed.
+
+  Lemma mx_one_spec n i j :
+    (mx_one bool_ops bool_tt n) i j <-> i = j.
+  Proof.
+    simpl. unfold mx_one.
+    unfold eqb_ord, ofbool, is_true. simpl.
+    split; ins; desf; desf.
+    now apply eq_ord.
+  Qed.
+
+  Theorem translate_slice'_spec' pi' i j r n_from
+    (Hwf' : PatternSlice.wf' (Rcd.type_of r) pi')
+    (Hij : translate_slice' pi' i j)
+    (Hprev : r n_from = Some (Value.GVertex i)) :
+      exists p', PathSlice.matches G r n_from r p' pi' /\
+                  PathSlice.last r n_from p' = j.
+  Proof using Hwf_G.
+    gen_dep j.
+    induction pi'; ins.
+    { exists PathSlice.empty. split.
+      { constructor. eexists; eassumption. }
+      rewrite mx_one_spec in Hij. simpl. desf. }
+
+    inv Hwf'. inv Hwf_G.
+    unfold mx_dot in *.
+
+    rewrite is_true_sup in Hij; destruct Hij as [j' [_ Hij]].
+    rewrite andb_is_true_iff in Hij; destruct Hij as [Hij Hj'j].
+
+    destruct (Pattern.vlabel pv) as [l |] eqn:Heq_v.
+    1: rewrite label_matrix_spec in Hj'j;
+        destruct Hj'j as [? Hvlabel].
+    2: rewrite mx_one_spec in Hj'j.
+    all: subst j'.
+
+    all: rewrite is_true_sup in Hij; destruct Hij as [k [_ Hij]].
+    all: rewrite andb_is_true_iff in Hij; destruct Hij as [Hik Hkj].
+
+    all: destruct (Pattern.edir pe) eqn:Heq_edir; simpls.
+    all: try rewrite adj_matrix_spec_OUT in Hkj.
+    all: try rewrite adj_matrix_spec_IN in Hkj.
+    all: try rewrite adj_matrix_spec_BOTH in Hkj.
+    all: apply IHpi' in Hik; clear IHpi'; auto.
+    all: desf.
+
+    all: exists (PathSlice.hop p' e j); split; [| reflexivity].
+    all: replace r with ((Pattern.vname pv, Pattern.ename pe) |-[Mixed]->
+                          (Value.GVertex j, Value.GEdge e); r) at 2
+                    by (simpl; unfold Name.is_implicit in *; desf).
+    all: constructor; auto.
+    all: try (left; apply Rcd.type_of_None;
+                eauto using PatternSlice.type_of_None).
+    all: try constructor.
+    all: try (ins; congruence).
+    all: try now rewrite Hik0, Heq_edir.
+
+    all: unfold Path.matches_direction in Hkj0; desf.
+    all: edestruct ends_In0; eauto.
+  Qed.
+
+  Theorem translate_slice'_spec r r' n_from p' pi' (i j : ord _) 
+    (Hwf' : PatternSlice.wf' (Rcd.type_of r) pi')
+    (Hprev : r n_from = Some (Value.GVertex i))
+    (HIn_prev : In (i : vertex) (vertices G))
+    (Hlast : PathSlice.last r n_from p' = j)
+    (Hmatch : PathSlice.matches G r n_from r' p' pi') :
+      translate_slice' pi' i j.
+  Proof.
+    gen_dep j; induction Hmatch; ins; subst.
+    { simpl. rewrite mx_one_spec. desf. now apply eq_ord. }
+    
+    assert (exists k : ord vertices_sup, PathSlice.last r n_from p = k) as [k Hk].
+    { enough (HIn : In (PathSlice.last r n_from p) (vertices G)).
+      now eexists (ord_of_vertex _ HIn).
+      eapply PathSlice.matches_last_In; eauto. }
+
+    assert (IH : translate_slice' pi i k).
+    { apply IHHmatch; auto. inv Hwf'. }
+    clear IHHmatch.
+    unfold mx_dot. desf.
+
+    all: rewrite is_true_sup.
+    all: exists j.
+    all: split; [ apply in_seq | ].
+    all: rewrite andb_is_true_iff.
+
+    all: try rewrite mx_one_spec.
+    all: try rewrite label_matrix_spec.
+    all: destruct Hpv.
+    all: splits; auto.
+
+    all: rewrite is_true_sup.
+    all: exists k.
+    all: split; [ apply in_seq | ].
+    all: rewrite andb_is_true_iff.
+    all: split; [ assumption | ].
+
+    all: simpl.
+    all: match goal with
+          | [ _ : _ = Pattern.OUT |- _ ] =>
+              rewrite adj_matrix_spec_OUT
+          | [ _ : _ = Pattern.IN |- _ ] =>
+              rewrite adj_matrix_spec_IN
+          | [ _ : _ = Pattern.BOTH |- _ ] =>
+              rewrite adj_matrix_spec_BOTH
+          end.
+    all: exists e.
+    all: destruct Hpe.
+    all: rewrite Hk in Hdir.
+    all: splits; auto.
+    all: desf; eauto.
+  Qed.
+End translate.
+
+
 Definition traverse : PatternSlice.t -> Name.t -> step1.
 Admitted.
 
-Theorem traverse_wf : forall graph table ty slice n_from,
-  PropertyGraph.wf graph -> BindingTable.of_type table ty ->
+Theorem traverse_wf : forall G table ty slice n_from,
+  PropertyGraph.wf G -> BindingTable.of_type table ty ->
     PatternSlice.wf ty slice -> ty n_from = Some Value.GVertexT ->
-      exists table', traverse slice n_from graph table = Some table'.
+      exists table', traverse slice n_from G table = Some table'.
 Admitted.
 
-Theorem traverse_type : forall graph table table' ty slice n_from,
-  traverse slice n_from graph table = Some table' ->
+Theorem traverse_type : forall G table table' ty slice n_from,
+  traverse slice n_from G table = Some table' ->
     BindingTable.of_type table ty ->
       BindingTable.of_type table' (PatternSlice.type_of ty slice).
 Admitted.
 
-Theorem traverse_spec : forall graph table table' path r r' slice n_from,
-  traverse slice n_from graph table = Some table' ->
-    PathSlice.matches graph r n_from r' path slice ->
+Theorem traverse_spec : forall G table table' path r r' slice n_from,
+  traverse slice n_from G table = Some table' ->
+    PathSlice.matches G r n_from r' path slice ->
       In r table -> In r' table'.
 Admitted.
 
-Theorem traverse_spec' : forall graph table table' r' slice n_from,
-  traverse slice n_from graph table = Some table' ->
+Theorem traverse_spec' : forall G table table' r' slice n_from,
+  traverse slice n_from G table = Some table' ->
     In r' table' -> exists r path, In r table /\
-      PathSlice.matches graph r n_from r' path slice.
+      PathSlice.matches G r n_from r' path slice.
 Admitted.
